---
layout: mathpost
title:  "6.832 Underactuated Robotics - Lecture 1"
mathjax: true
tags: [math, control, robotics]
local: false
---
## [Video Lecture](https://youtu.be/VeEqtTgDXFc) | [Class Notes](http://underactuated.csail.mit.edu/intro.html)

## [Problem Set](http://underactuated.csail.mit.edu/Spring2019/set_1.zip)

# 1.1.1
Underactuated, because a purely `sideways' acceleration in the direction opposing
gravity is not possible for any control input.
So the map $\ddot q = f(q, \dot q, u, t)$ is not surjective.

# 1.1.2
If we assume unit mass, length and inertia matrix, 
$$
\begin{bmatrix}\ddot x \\ \ddot z + g \\ \ddot \theta\end{bmatrix} =
\begin{bmatrix}
-sin \theta & -sin \theta \\
cos \theta & cos \theta \\
1 & -1
\end{bmatrix} \begin{bmatrix}F_1 \\ F_2\end{bmatrix}
$$
i.e. system is control affine.

Let us take the example of a purely sideways acceleration i.e.
$$
\begin{align*}
& \ddot \theta = 0, \ddot x = a cos \theta, \ddot z = a sin \theta\\
&\implies F_1 = F_2 = k (say)\\
&\implies a cos \theta = -2k sin \theta, a sin \theta + g = 2k cos \theta\\
&\implies a = -g sin \theta
\end{align*}
$$

For $\theta = 0.5$, $sin \theta \approx 0.5$. Hence $a$ cannot be positive.
Concretely, $\ddot q = (5 cos \theta, 5 sin \theta, 0)$ is not possible
instantaneously at $\theta = 0.5$.

# 1.2.1

In this case,

$$
\begin{align*}
f_r &= K_1\\
f_f &= K_2 - C_f \phi\\
I\ddot \theta &= -b f_r + a f_f cos \phi\\
&= -bK_1 + a K_2 cos \phi - a C_f \phi cos \phi\\
m \ddot x &= K_3 - f_f sin(\theta + \phi) + u_r cos \theta\\
&= K_3 - K_2 sin(\theta + \phi) + C_f \phi sin(\theta + \phi) + u_r cos \theta\\ 
m \ddot y &= K_4 + f_f cos(\theta + \phi) + u_r sin \theta\\
&= K_4 + K_2 cos(\theta + \phi) - C_f \phi cos(\theta + \phi) + u_r sin \theta\\
\implies
\begin{bmatrix}I\ddot \theta \\ m \ddot x\\ m \ddot y\end{bmatrix} &=
\begin{bmatrix}
-bK_1 + a K_2 cos \phi\\
K_3 - K_2 sin(\theta + \phi)\\
K_4 + K_2 cos(\theta + \phi)
\end{bmatrix} +
\begin{bmatrix}
-a C_f cos \phi & 0\\
C_f sin(\theta + \phi) & cos \theta\\
-C_f cos(\theta + \phi) & sin \theta 
\end{bmatrix}
\begin{bmatrix}\phi \\ u_r\end{bmatrix}
\end{align*}
$$

which means the system is control-affine. The $B$ matrix has shape 2 $\times$ 3,
while dim($q$) = 3, which means the system is underactuated.

# 1.2.2

Intuitively, the system is still underactuated because of holonomic constraints.
An acceleration of the type $(\ddot x, \ddot y, \ddot \theta) = (0, k, 0)$ is
not possible instantaneously.

# 1.2.3

When $\phi_0 = 0$

$$
f_2(q, \dot q, t) =
\begin{bmatrix}
-a C_f & 0 & 0\\
-C_f arctan\left( \frac{\dot y + \dot \theta a}{\dot x} \right) & 1 & 1\\
-C_f & 0 & 0
\end{bmatrix}
$$

which has rank 2 because rows 1 and 2 are not linearly independent.

# 1.2.4

row 1 = $a \times$ row 3, so they will never be linearly independent. Hence there
are no values of $\phi_0$ for which the linearized system is fully actuated.

# 1.3.1

1. No, we need the position and velocity of center of mass (or any other
well defined point on the robot body) in the state as well.
2. False, because no control input can produce a (large) vertical acceleration in the
COM.
3. False, because pure in-place rotation acceleration of the COM or acceleration the COM
along the straight line are not possible.

## Deriving the Manipulator Equations
State $q = \begin{bmatrix}\theta_1 \\\ \theta_2\end{bmatrix}$.

Positions of masses $m_1$ and $m_2$ are:

$$
p_1 = l_1\begin{bmatrix}s_1 \\\ -c_1 \end{bmatrix}
$$

$$
p_2 = p_1 + l_2\begin{bmatrix}s_{1+2} \\\ -c_{1+2} \end{bmatrix}
$$

Velocities are:

$$
\dot p_1 = l_1 \dot\theta_1 \begin{bmatrix}c_1 \\\ s_1 \end{bmatrix}
$$

$$
\dot p_2 = \dot p_1 + l_2 \left(\dot\theta_1 + \dot\theta_2\right) \begin{bmatrix}c_{1+2} \\\ s_{1+2} \end{bmatrix}
$$

Total kinetic energy

$$
\begin{align*}
T &= \frac{1}{2}m_1 \dot p_1^T \dot p_1 + \frac{1}{2}m_2 \dot p_2^T \dot p_2\\
&= \frac{1}{2}m_1 \dot p_1^T \dot p_1 +
\frac{1}{2}m_2 \left(
    \dot p_1^T \dot p_1 +
    2 l_2 \left(\dot\theta_1 + \dot\theta_2\right) \dot p_1^T \begin{bmatrix}c_{1+2} \\\ s_{1+2} \end{bmatrix} +
    l_2^2 \left(\dot\theta_1 + \dot\theta_2\right)^2
\right)\\
&= \frac{1}{2} (m_1 + m_2) l_1^2 \dot \theta_1^2 +
m_2 l_1 l_2 \dot\theta_1 \left(\dot\theta_1 + \dot\theta_2\right) (c_1 c_{1+2} + s_1 s_{1+2}) +
\frac{1}{2} m_2 l_2^2 \left(\dot\theta_1 + \dot\theta_2\right)^2 \\
&= \frac{1}{2} (m_1 + m_2) l_1^2 \dot \theta_1^2 +
c_2 m_2 l_1 l_2 \dot\theta_1 \left(\dot\theta_1 + \dot\theta_2\right)+
\frac{1}{2} m_2 l_2^2 \left(\dot\theta_1 + \dot\theta_2\right)^2
\end{align*}
$$

Total potential energy

$$
\begin{align*}
U &= m_1 g y_1 + m_2 g y_2\\
&=-g\left(m_1 l_1 c_1 + m_2(l_1 c_1 + l_2 c_{1+2}) \right)
\end{align*}
$$

The Lagrangian is $L = T - U$

# [Lagrangian equation of the first kind](https://en.wikipedia.org/wiki/Lagrangian_mechanics) for $\theta_1$:

$$
\dv{}{t} \pdv{L}{\dot \theta_1} - \pdv{L}{\theta_1} = \tau_1
$$

Now 

$$
\begin{align*}
\pdv{L}{\dot \theta_1}
&= \pdv{}{\dot \theta_1} \left[ \frac{1}{2} (m_1 + m_2) l_1^2 \dot \theta_1^2 +
c_2 m_2 l_1 l_2 \dot\theta_1 \left(\dot\theta_1 + \dot\theta_2\right)+
\frac{1}{2} m_2 l_2^2 \left(\dot\theta_1 + \dot\theta_2\right)^2 + 
g\left(m_1 l_1 c_1 + m_2(l_1 c_1 + l_2 c_{1+2}) \right) \right]\\
&= (m_1 + m_2) l_1^2 \dot \theta_1 +
c_2 m_2 l_1 l_2 (2\dot\theta_1 + \dot\theta_2) +
m_2 l_2^2 \left(\dot\theta_1 + \dot\theta_2\right)
\end{align*}
$$

Hence 

$$
\begin{align*}
\dv{}{t} \pdv{L}{\dot \theta_1}
&= \dv{}{t} \left[ (m_1 + m_2) l_1^2 \dot \theta_1 +
c_2 m_2 l_1 l_2 (2\dot\theta_1 + \dot\theta_2) +
m_2 l_2^2 \left(\dot\theta_1 + \dot\theta_2\right) \right] \\
&= (m_1 + m_2) l_1^2 \ddot \theta_1 +
m_2 l_2^2 \left(\ddot\theta_1 + \ddot\theta_2\right) +
m_2 l_1 l_2 (2\ddot\theta_1 + \ddot\theta_2) c_2 -
m_2 l_1 l_2 (2\dot\theta_1 + \dot\theta_2) \dot \theta_2 s_2  
\end{align*}
$$

And

$$
\begin{align*}
\pdv{L}{\theta_1}
&= \pdv{}{\theta_1} \left[ \frac{1}{2} (m_1 + m_2) l_1^2 \dot \theta_1^2 +
c_2 m_2 l_1 l_2 \dot\theta_1 \left(\dot\theta_1 + \dot\theta_2\right)+
\frac{1}{2} m_2 l_2^2 \left(\dot\theta_1 + \dot\theta_2\right)^2 + 
g\left(m_1 l_1 c_1 + m_2(l_1 c_1 + l_2 c_{1+2}) \right) \right]\\
&= -g \left(m_1 l_1 s_1 + m_2 \left(l_1 s_1 + l_2 s_{1+2} \right) \right) \\
&= -(m_1 + m_2) l_1 g s_1 - m_2 g l_2 s_{1+2}
\end{align*}
$$

Hence we get the Lagrangian equation

$$
\begin{equation*}
\boxed{
(m_1 + m_2) l_1^2 \ddot \theta_1 +
m_2 l_2^2 \left(\ddot\theta_1 + \ddot\theta_2\right) +
m_2 l_1 l_2 (2\ddot\theta_1 + \ddot\theta_2) c_2 -
m_2 l_1 l_2 (2\dot\theta_1 + \dot\theta_2) \dot \theta_2 s_2 +
(m_1 + m_2) l_1 g s_1 +
m_2 g l_2 s_{1+2} = \tau_1
}
\end{equation*}
$$

# Similarly, [Lagrangian equation of the first kind](https://en.wikipedia.org/wiki/Lagrangian_mechanics) for $\theta_2$:

$$
\dv{}{t} \pdv{L}{\dot \theta_2} - \pdv{L}{\theta_2} = \tau_2
$$ 

Now 

$$
\begin{align*}
\pdv{L}{\dot \theta_2}
&= \pdv{}{\dot \theta_2} \left[ \frac{1}{2} (m_1 + m_2) l_1^2 \dot \theta_1^2 +
c_2 m_2 l_1 l_2 \dot\theta_1 \left(\dot\theta_1 + \dot\theta_2\right)+
\frac{1}{2} m_2 l_2^2 \left(\dot\theta_1 + \dot\theta_2\right)^2 + 
g\left(m_1 l_1 c_1 + m_2(l_1 c_1 + l_2 c_{1+2}) \right) \right]\\ 
&= c_2 m_2 l_1 l_2 \dot\theta_1 +
m_2 l_2^2 \left(\dot\theta_1 + \dot\theta_2\right) 
\end{align*}
$$

Hence

$$
\begin{align*}
\dv{}{t} \pdv{L}{\dot \theta_2}
&= \dv{}{t} \left[ c_2 m_2 l_1 l_2 \dot\theta_1 +
m_2 l_2^2 \left(\dot\theta_1 + \dot\theta_2\right) \right] \\
&= c_2 m_2 l_1 l_2 \ddot\theta_1 -
s_2 m_2 l_1 l_2 \dot\theta_1 \dot\theta_2 +
m_2 l_2^2 \left(\ddot\theta_1 + \ddot\theta_2\right)
\end{align*}
$$

And

$$
\begin{align*}
\pdv{L}{\theta_2}
&= \pdv{}{\theta_2} \left[ \frac{1}{2} (m_1 + m_2) l_1^2 \dot \theta_1^2 +
c_2 m_2 l_1 l_2 \dot\theta_1 \left(\dot\theta_1 + \dot\theta_2\right) +
\frac{1}{2} m_2 l_2^2 \left(\dot\theta_1 + \dot\theta_2\right)^2 + 
g\left(m_1 l_1 c_1 + m_2(l_1 c_1 + l_2 c_{1+2}) \right) \right]\\
&= -s_2 m_2 l_1 l_2 \dot\theta_1 \left(\dot\theta_1 + \dot\theta_2\right) -
g m_2 l_2 s_{1+2}
\end{align*}
$$

Hence we get the Lagrangian equation

$$
c_2 m_2 l_1 l_2 \ddot\theta_1 -
s_2 m_2 l_1 l_2 \dot\theta_1 + \dot\theta_2
m_2 l_2^2 \left(\ddot\theta_1 + \ddot\theta_2\right) +
s_2 m_2 l_1 l_2 \dot\theta_1 \left(\dot\theta_1 + \dot\theta_2\right) +
g m_2 l_2 s_{1+2} = \tau_2
$$

$$
\begin{equation*}
\boxed{\implies
m_2 l_2^2 \left(\ddot\theta_1 + \ddot\theta_2\right) +
m_2 l_1 l_2 \ddot\theta_1 c_2 +
m_2 l_1 l_2 \dot\theta_1^2 +
m_2 g l_2 s_{1+2} = \tau_2
}
\end{equation*}
$$

The Lagrangian equations match the [notes](http://underactuated.csail.mit.edu/multibody.html#example1)
and follow the canonical form of manipulator equations

$$
M(q) \ddot q + C(q, \dot q)\dot q = \tau_g(q) + Bu
$$